src/Lean/Elab/Tactic/Do/ProofMode/Intro.lean
@@ -15,32 +15,32 @@ namespace Lean.Elab.Tactic.Do.ProofMode
 open Std.Do SPred.Tactic
 open Lean Elab Tactic Meta
 
-partial def mIntro [Monad m] [MonadControlT MetaM m] [MonadLiftT MetaM m] (goal : MGoal) (ident : TSyntax ``binderIdent) (k : MGoal → m (α × Expr)) : m (α × Expr) := do
+partial def mIntro [Monad m] [MonadControlT MetaM m] [MonadLiftT MetaM m] (goal : MGoal) (ident : TSyntax ``binderIdent) (k : MGoal → m Expr) : m Expr := do
   if let some (σs, H, T) := goal.target.app3? ``SPred.imp then
-  let (name, ref) ← liftMetaM <| getFreshHypName ident
-  let uniq ← liftMetaM mkFreshId
-  let hyp := Hyp.mk name uniq H
-  addHypInfo ref σs hyp (isBinder := true)
-  let Q := goal.hyps
-  let H := hyp.toExpr
-  let (P, hand) := mkAnd goal.u goal.σs goal.hyps H
-  let (a, prf) ← k { goal with hyps := P, target := T }
-  let prf := mkApp7 (mkConst ``Intro.intro [goal.u]) σs P Q H T hand prf
-  return (a, prf)
+    let (name, ref) ← liftMetaM <| getFreshHypName ident
+    let uniq ← liftMetaM mkFreshId
+    let hyp := Hyp.mk name uniq H
+    addHypInfo ref σs hyp (isBinder := true)
+    let Q := goal.hyps
+    let H := hyp.toExpr
+    let (P, hand) := SPred.mkAnd goal.u goal.σs goal.hyps H
+    let prf ← k { goal with hyps := P, target := T }
+    let prf := mkApp7 (mkConst ``Intro.intro [goal.u]) σs P Q H T hand prf
+    return prf
   else if let .letE name type val body _nondep := goal.target then
     let name ← match ident with
     | `(binderIdent| $name:ident) => pure name.getId
     | `(binderIdent| $_) => liftMetaM <| mkFreshUserName name
     -- Even if `_nondep = true` we want to retain the value of the let binding for the proof.
     withLetDecl name type val (nondep := false) fun val => do
-      let (a, prf) ← k { goal with target := body.instantiate1 val }
+      let prf ← k { goal with target := body.instantiate1 val }
       let prf ← liftMetaM <| mkLetFVars #[val] prf
-      return (a, prf)
+      return prf
   else
     liftMetaM <| throwError "Target not an implication or let-binding {goal.target}"
 
 -- This is regular MVar.intro, but it takes care not to leave the proof mode by preserving metadata
-partial def mIntroForall [Monad m] [MonadControlT MetaM m] [MonadLiftT MetaM m] (goal : MGoal) (ident : TSyntax ``binderIdent) (k : MGoal → m (α × Expr)) : m (α × Expr) :=
+partial def mIntroForall [Monad m] [MonadControlT MetaM m] [MonadLiftT MetaM m] (goal : MGoal) (ident : TSyntax ``binderIdent) (k : MGoal → m Expr) : m Expr :=
   controlAt MetaM fun map => do
   let some (_type, σ, σs') := (← whnf goal.σs).app3? ``List.cons | liftMetaM <| throwError "Ambient state list not a cons {goal.σs}"
   let name ← match ident with
@@ -51,11 +51,11 @@ partial def mIntroForall [Monad m] [MonadControlT MetaM m] [MonadLiftT MetaM m] 
     let H := pushForallContextIntoHyps σs' (mkApp goal.hyps s)
     let T := goal.target.betaRev #[s]
     map do
-      let (a, prf) ← k { u := goal.u, σs:=σs', hyps:=H, target:=T }
+      let prf ← k { u := goal.u, σs:=σs', hyps:=H, target:=T }
       let prf ← mkLambdaFVars #[s] prf
-      return (a, mkApp5 (mkConst ``SPred.entails_cons_intro [goal.u]) σs' σ goal.hyps goal.target prf)
+      return mkApp5 (mkConst ``SPred.entails_cons_intro [goal.u]) σs' σ goal.hyps goal.target prf
 
-def mIntroForallN [Monad m] [MonadControlT MetaM m] [MonadLiftT MetaM m] (goal : MGoal) (n : Nat) (k : MGoal → m (α × Expr)) : m (α × Expr) :=
+def mIntroForallN [Monad m] [MonadControlT MetaM m] [MonadLiftT MetaM m] (goal : MGoal) (n : Nat) (k : MGoal → m Expr) : m Expr :=
   match n with
   | 0 => k goal
   | n+1 => do mIntroForall goal (← liftMetaM `(binderIdent| _)) fun g =>
@@ -76,18 +76,18 @@ def elabMIntro : Tactic
     let (mvar, goal) ← mStartMVar (← getMainGoal)
     mvar.withContext do
     let goals ← IO.mkRef []
-    mvar.assign (← Prod.snd <$> mIntro goal ident fun newGoal => do
+    mvar.assign (← mIntro goal ident fun newGoal => do
       let m ← mkFreshExprSyntheticOpaqueMVar newGoal.toExpr
       goals.modify (m.mvarId! :: ·)
-      return ((), m))
+      return m)
     replaceMainGoal (← goals.get)
   | `(tactic| mintro ∀$ident:binderIdent) => do
     let (mvar, goal) ← mStartMVar (← getMainGoal)
     mvar.withContext do
     let goals ← IO.mkRef []
-    mvar.assign (← Prod.snd <$> mIntroForall goal ident fun newGoal => do
+    mvar.assign (← mIntroForall goal ident fun newGoal => do
       let m ← mkFreshExprSyntheticOpaqueMVar newGoal.toExpr
       goals.modify (m.mvarId! :: ·)
-      return ((), m))
+      return m)
     replaceMainGoal (← goals.get)
   | _ => throwUnsupportedSyntax
