src/Lean/Elab/Tactic/Do/ProofMode/Revert.lean
@@ -70,7 +70,7 @@ partial def mRevertForallN (goal : MGoal) (n : Nat) (hypName : Name) (k : MGoal 
   let σs' := revertArgsTypes.foldr (TypeList.mkCons u) goal.σs
   let H ← instantiateMVarsIfMVarApp H
   let H := pushForallContextIntoHyps σs' H
-  let (H, hand) := mkAnd u σs' H φ
+  let (H, hand) := SPred.mkAnd u σs' H φ
 
   -- Prove `((fun s₁ ... sₙ => H) ∧ (fun s₁ ... sₙ => ⌜s₁ = e₁ ∧ ... ∧ sₙ = eₙ⌝)) ⊢ₛ T`
   let goal' := { u, σs := σs', hyps := H, target := mkAppRev f args[n:] }
