src/Lean/Meta/Tactic/FunInd.lean
@@ -319,7 +319,7 @@ partial def foldAndCollect (oldIH newIH : FVarId) (isRecCall : Expr → Option E
             -- statement and the inferred alt types
             let dummyGoal := mkConst ``True []
             mkArrow eTypeAbst dummyGoal)
-          (onAlt := fun _altIdx altType alt => do
+          (onAlt := fun _altIdx altType _altParams alt => do
             lambdaTelescope1 alt fun oldIH' alt => do
               forallBoundedTelescope altType (some 1) fun newIH' _goal' => do
                 let #[newIH'] := newIH' | unreachable!
@@ -337,7 +337,7 @@ partial def foldAndCollect (oldIH newIH : FVarId) (isRecCall : Expr → Option E
           (onMotive := fun _motiveArgs motiveBody => do
             let some (_extra, body) := motiveBody.arrow? | throwError "motive not an arrow"
             M.eval (foldAndCollect oldIH newIH isRecCall body))
-          (onAlt := fun _altIdx altType alt => do
+          (onAlt := fun _altIdx altType _altParams alt => do
             lambdaTelescope1 alt fun oldIH' alt => do
             -- We don't have suitable newIH around here, but we don't care since
             -- we just want to fold calls. So lets create a fake one.
@@ -846,19 +846,19 @@ partial def buildInductionBody (toErase toClear : Array FVarId) (goal : Expr)
 
   -- match and casesOn application cause case splitting
   if let some matcherApp ← matchMatcherApp? e (alsoCasesOn := true) then
-    -- Calculate motive
-    let eType ← newIH.getType
-    let motiveBody ← mkArrow eType goal
-    let (mask, absMotiveBody) ← mkLambdaFVarsMasked matcherApp.discrs motiveBody
-
     -- A match that refines the parameter has been modified by `Fix.lean` to refine the IH,
     -- so we need to replace that IH
     if matcherApp.remaining.size == 1 && matcherApp.remaining[0]!.isFVarOf oldIH then
+      -- Calculate motive
+      let eType ← newIH.getType
+      let motiveBody ← mkArrow eType goal
+      let (mask, absMotiveBody) ← mkLambdaFVarsMasked matcherApp.discrs motiveBody
+
       let matcherApp' ← matcherApp.transform (useSplitter := true)
         (addEqualities := true)
         (onParams := (foldAndCollect oldIH newIH isRecCall ·))
         (onMotive := fun xs _body => pure (absMotiveBody.beta (maskArray mask xs)))
-        (onAlt := fun altIdx expAltType alt => M2.branch do
+        (onAlt := fun altIdx expAltType _altParams alt => M2.branch do
           lambdaTelescope1 alt fun oldIH' alt => do
             forallBoundedTelescope expAltType (some 1) fun newIH' goal' => do
               let #[newIH'] := newIH' | unreachable!
@@ -881,7 +881,7 @@ partial def buildInductionBody (toErase toClear : Array FVarId) (goal : Expr)
         (addEqualities := true)
         (onParams := (foldAndCollect oldIH newIH isRecCall ·))
         (onMotive := fun xs _body => pure (absMotiveBody.beta (maskArray mask xs)))
-        (onAlt := fun altIdx expAltType alt => M2.branch do
+        (onAlt := fun altIdx expAltType _altParams alt => M2.branch do
           withRewrittenMotiveArg expAltType (rwMatcher altIdx) fun expAltType' =>
             buildInductionBody toErase toClear expAltType' oldIH newIH isRecCall alt)
       return matcherApp'.toExpr
